src/cbor/pulse/CBOR.Pulse.API.Nondet.C.fsti
@@ -155,3 +155,7 @@ val cbor_nondet_mk_map_entry (_: unit) : mk_map_entry_t #_ #_ cbor_nondet_match 
 
 val cbor_nondet_mk_map (_: unit)
 : mk_map_from_arrayptr_safe_t #cbor_nondet_t #cbor_nondet_map_entry_t cbor_nondet_match cbor_nondet_map_entry_match
+
+type cbor_nondet_map_get_multiple_entry_t = cbor_map_get_multiple_entry_t cbor_nondet_t
+
+val cbor_nondet_map_get_multiple (_: unit) : cbor_map_get_multiple_as_arrayptr_t #_ cbor_nondet_match cbor_nondet_map_get_multiple_entry_t
