src/cbor/pulse/CBOR.Pulse.API.Nondet.Rust.fsti
@@ -149,3 +149,5 @@ val cbor_nondet_mk_map_entry (_: unit) : mk_map_entry_t #_ #_ cbor_nondet_match 
 
 val cbor_nondet_mk_map_gen (_: unit)
 : mk_map_gen_by_ref_t #cbor_nondet_t #cbor_nondet_map_entry_t cbor_nondet_match cbor_nondet_map_entry_match
+
+val cbor_nondet_map_get_multiple (_: unit) : cbor_map_get_multiple_t #_ cbor_nondet_match
